src/Preservation.v
@@ -12,7 +12,39 @@ Require Maps.
 Import Maps.Notations.
 
 
-Theorem preservation : ∀ e e' t,
+
+
+(* Theorem preservation : ∀ e e' t,
+  has_type empty e t  ->
+  step e e'  ->
+  has_type empty e' t.
+Proof.
+  (* remember empty as Γ. *)
+  (* induction e;
+  intros * H_type_e H_step.
+  - inversion H_type_e. discriminate H1.
+  - inversion H_type_e; subst. 
+    inversion H_step; subst; eauto with local_hints.
+    inversion H4; subst.
+    eapply Step.subst_typing; eauto.
+  -   *)
+
+  induction e; intros e' τ H_type H_step;
+  try (inversion H_type; subst; 
+    inversion H_step; subst;
+    eauto with local_hints).
+    - inversion H4. eauto with local_hints.
+    - inversion H2; subst. 
+      rewrite Maps.update_eq in H4. 
+      inversion H4; subst. auto.
+    - inversion H2; subst. 
+      inversion H5; subst.
+      + eapply T_Access.
+
+    
+Qed. *)
+
+(* Theorem preservation : ∀ e e' t,
   has_type empty e t  ->
   step e e'  ->
   has_type empty e' t.
@@ -27,33 +59,11 @@ Proof.
     subst; 
     eauto with local_hints).
   - inversion H_type_e2; subst. eauto with local_hints.
-  - apply T_Rec.
-    inversion H_step; subst.
-    assert (Maps.same_bindings (x |-> e'0; m) (x |-> e; m)).
-    {
-      apply Maps.same_bindings_update.
-      apply Maps.same_bindings_refl.
-    }
-    eapply Maps.same_bindings_trans; eauto.
-Qed.
-
-Theorem preservation' : ∀ e e' t,
-  has_type empty e t  ->
-  step e e'  ->
-  has_type empty e' t.
-Proof.
-  induction e; intros e' τ H_type H_step;
-  try (inversion H_type; subst; 
-    inversion H_step; subst;
-    eauto with local_hints).
-    - inversion H4. eauto with local_hints.
-    - apply T_Rec.
-      inversion H_step; subst.
-      assert (Maps.same_bindings (x |-> e'0; fields) fields).
-      {
-        eapply Maps.same_bindings_shadow_add.
-        - apply Maps.same_bindings_refl.
-        - apply H5. 
-      }
-      eapply Maps.same_bindings_trans; eauto.
-Qed.
+  - inversion H_type_e; subst. 
+    inversion H. rewrite String.eqb_refl in H1. 
+    inversion H1; subst. auto.
+  - inversion H6; subst.
+    + eapply Step.not_value in H4. exfalso. eauto.
+    + admit.
+    + 
+Qed. *)
