src/Subst.v
@@ -59,18 +59,19 @@ Inductive substitution (s : expr) (x : string) : expr -> expr -> Prop :=
         substitution s x e1 e1' -> 
         substitution s x e2 e2' -> 
         substitution s x (E_Minus e1 e2) (E_Minus e1' e2')
-    | S_Rec_Unit : 
-        substitution s x (E_Rec Maps.empty) (E_Rec Maps.empty)
-
-    | S_Rec_Rec :
-        ∀ m m' y e e', 
-        substitution s x (E_Rec m) (E_Rec m') ->
-        substitution s x e e' ->
-        substitution s x (E_Rec (y |-> e; m)) (E_Rec (y |-> e'; m'))
-    | S_Access :
-        ∀ e e' y, 
-        substitution s x e e' ->
-        substitution s x (E_Access e y) (E_Access e' y)
+    | S_Pair : 
+        ∀ (e1 e1' e2 e2': expr),
+        substitution s x e1 e1' -> 
+        substitution s x e2 e2' -> 
+        substitution s x (E_Pair e1 e2) (E_Pair e1' e2')
+    | S_First :
+        ∀ (e e': expr),
+        substitution s x e e' -> 
+        substitution s x (E_First e) (E_First e')
+    | S_Second :
+        ∀ (e e': expr),
+        substitution s x e e' -> 
+        substitution s x (E_Second e) (E_Second e')
 .
 
 Hint Constructors substitution : local_hints.
@@ -87,11 +88,6 @@ Proof with eauto with local_hints.
     try destruct (String.eqb_spec x x0); 
     subst;
     eauto with local_hints; fail).
-Admitted.
-    (* induction fields...
-    inversion IHfields as [e' H_subst].
-    inversion H_subst; subst.
-    -  
-Qed. *)
+Qed.
 
 Hint Resolve exists_one : local_hints.
